Prove lambda calculus lists correct

parse.ml
@@ -1,0 +1,218 @@
+type lam_tree =
+  | Lam_end
+  | Lam_lam of lam_tree
+  | Lam_dot of  lam_tree
+  | Lam_out of lam_tree
+  | Lam_wsp of lam_tree
+  | Lam_id of string * lam_tree
+  | Lam_paren of lam_tree * lam_tree
+
+type parse_state =
+  | Ok of lam_tree * (lam_tree list)
+  | Error
+
+
+let rec parse_lambdatree_state (l: char list): parse_state =
+    match l with
+    | [] -> Ok (Lam_end, [])
+    | hd :: tl ->
+      (match parse_lambdatree_state tl with
+       | Error -> Error
+       | Ok (cur, stack) ->
+          (match hd with
+           | ' ' | '\t' | '\n' ->
+              (match cur with
+               | Lam_wsp _ -> Ok (cur, stack)
+               | _ -> Ok ((Lam_wsp cur), stack))
+           | '\\' -> Ok ((Lam_lam cur), stack)
+           | '.' -> Ok ((Lam_dot cur), stack)
+           | '^' -> Ok ((Lam_out cur), stack)
+           | ')' -> Ok ((Lam_end), (cur :: stack))
+           | '(' ->
+              (match stack with
+               | [] -> Error
+               | next :: stack' -> Ok ((Lam_paren cur next), stack'))
+           | _ ->
+              (match cur with
+               | Lam_id str next -> Ok ((Lam_id (String hd str) next), stack)
+               | _ -> Ok ((Lam_id (String hd EmptyString) cur), stack))))
+
+let rec lambda_strip_wsp (t: Lam_tree): Lam_tree =
+    match t with
+    | Lam_end -> Lam_end
+    | Lam_wsp t' -> lambda_strip_wsp t'
+    | Lam_lam t' -> Lam_lam (lambda_strip_wsp t')
+    | Lam_dot t' -> Lam_dot (lambda_strip_wsp t')
+    | Lam_out t' -> Lam_out (lambda_strip_wsp t')
+    | Lam_id s t' -> Lam_id s (lambda_strip_wsp t')
+    | Lam_paren inner t' ->
+      Lam_paren (lambda_strip_wsp inner) (lambda_strip_wsp t')
+    end.
+
+  Local Inductive NamedLambda : Set =
+  | nl_var (s: string)
+  | nl_lam (s: string) (e: NamedLambda)
+  | nl_out (e: NamedLambda)
+  | nl_app (e1: NamedLambda) (e2: NamedLambda).
+
+  Function app_of_lambda_list (ls: list NamedLambda) {measure List.length ls}:
+    option NamedLambda =
+    match ls with
+    | [] -> None
+    | e :: [] -> Some e
+    | e1 :: e2 :: tl -> app_of_lambda_list ((nl_app e1 e2) :: tl)
+    end.
+  intuition.
+  Defined.
+
+  Function named_lambda_of_tree (acc: list NamedLambda) (t: lam_tree):
+    option NamedLambda =
+    match t with
+    | lam_end -> app_of_lambda_list (rev acc)
+    | lam_wsp _ -> None
+    | lam_lam (lam_id s (lam_dot t')) ->
+      match named_lambda_of_tree [] t' with
+      | None -> None
+      | Some e -> Some (nl_lam s e)
+      end
+    | lam_lam _ | lam_dot _ -> None
+    | lam_out t' ->
+      match named_lambda_of_tree [] t' with
+      | None -> None
+      | Some e -> Some (nl_out e)
+      end
+    | lam_id s t' -> named_lambda_of_tree (nl_var s :: acc) t'
+    | lam_paren inner t' ->
+      match named_lambda_of_tree [] inner with
+      | None -> None
+      | Some e -> named_lambda_of_tree (e :: acc) t'
+      end
+    end.
+
+  Function parse_named_lambda (s: string): option NamedLambda =
+    match parse_lambdatree_state (Parse.chars_of_string s) with
+    | Error -> None
+    | Ok cur stack ->
+      match stack with
+      | _ :: _ -> None
+      | [] -> named_lambda_of_tree [] (lambda_strip_wsp cur)
+      end
+    end.
+
+  Example named_id: parse_named_lambda "\x.x" = Some (nl_lam "x" (nl_var "x")).
+  auto. Qed.
+
+  Example named_true:
+    parse_named_lambda "\x.\y.x" = Some (nl_lam "x" (nl_lam "y" (nl_var "x"))).
+  auto. Qed.
+
+  Example named_false:
+    parse_named_lambda " \ x . \ y  .  (y  ) " =
+    Some (nl_lam "x" (nl_lam "y" (nl_var "y"))).
+  auto. Qed.
+
+  Example named_out:
+    parse_named_lambda "\x.^x" = Some (nl_lam "x" (nl_out (nl_var "x"))).
+  auto. Qed.
+
+  Example named_Y:
+    parse_named_lambda "\f.(\x.f (x x)) (\x.f (x x))" =
+    let fn_app = nl_app (nl_var "f") (nl_app (nl_var "x") (nl_var "x")) in
+    Some (nl_lam "f" (nl_app (nl_lam "x" fn_app) (nl_lam "x" fn_app))).
+  auto. Qed.
+
+  Example named_parens:
+    parse_named_lambda "(((\x.(((x))))))" = Some (nl_lam "x" (nl_var "x")).
+  auto. Qed.
+
+  Example named_apps:
+    parse_named_lambda "x y z w" =
+    Some (nl_app (
+              nl_app (
+                  nl_app (nl_var "x") (nl_var "y")
+                ) (nl_var "z")
+            ) (nl_var "w")).
+  auto. Qed.
+
+  Example named_bad_lambdas: parse_named_lambda "\\x.x" = None.
+  auto. Qed.
+
+  Example named_bad_dots: parse_named_lambda "\x..x" = None.
+  auto. Qed.
+
+  Example named_bad_parens: parse_named_lambda "\x.((x)" = None.
+  auto. Qed.
+
+  Example named_bad_parens2: parse_named_lambda "\x.x ()" = None.
+  auto. Qed.
+
+  Function index_of (x: string) (l: list string): option nat =
+    match l with
+    | [] -> None
+    | hd :: tl ->
+      if string_dec hd x then Some 0
+      else match index_of x tl with
+           | Some i -> Some (S i)
+           | None -> None
+           end
+    end.
+
+  Function lambda_strip_names (l: NamedLambda) (xs: list string):
+    option Lambda =
+    match l with
+    | nl_var x ->
+      match index_of x xs with
+      | Some n -> Some (l_var n)
+      | None -> None
+      end
+    | nl_lam x e ->
+      match lambda_strip_names e (x :: xs) with
+      | Some e' -> Some (l_lam e')
+      | None -> None
+      end
+    | nl_out e ->
+      match lambda_strip_names e xs with
+      | Some e' -> Some (l_out e')
+      | None -> None
+      end
+    | nl_app e1 e2 ->
+      match (lambda_strip_names e1 xs, lambda_strip_names e2 xs) with
+      | (Some e1', Some e2') -> Some (l_app e1' e2')
+      | _ -> None
+      end
+    end.
+
+  Function parse_lambda (s: string): option Lambda =
+    match parse_named_lambda s with
+    | None -> None
+    | Some nl -> lambda_strip_names nl []
+    end.
+
+  Example lambda_id: parse_lambda "\x.x" = Some (l_lam (l_var 0)).
+  auto. Qed.
+
+  Example lambda_true:
+    parse_lambda "\x.\y.x" = Some (l_lam (l_lam (l_var 1))).
+  auto. Qed.
+
+  Example lambda_false:
+    parse_lambda " \ x . \ y  .  (y  ) " =  Some (l_lam (l_lam (l_var 0))).
+  auto. Qed.
+
+  Example lambda_out:
+    parse_lambda "\x.^x" = Some (l_lam (l_out (l_var 0))).
+  auto. Qed.
+
+  Example lambda_Y:
+    parse_lambda "\f.(\x.f (x x)) (\x.f (x x))" =
+    let fn_app = l_app (l_var 1) (l_app (l_var 0) (l_var 0)) in
+    Some (l_lam (l_app (l_lam fn_app) (l_lam fn_app))).
+  auto. Qed.
+
+  Example lambda_parens:
+    parse_lambda "(((\x.(((x))))))" = Some (l_lam (l_var 0)).
+  auto. Qed.
+
+  Example lambda_apps:
+    parse_lambda "x y z w" = None.
+  auto. Qed.
