lambda.v
@@ -11,542 +11,555 @@ Import ListNotations.
 
 Load parse.
 
-(* Lambda Calculus with 0-indexed De Bruijn indices *)
-Inductive Lambda : Set :=
-| l_var : nat -> Lambda
-| l_out : Lambda -> Lambda
-| l_lam : Lambda -> Lambda
-| l_app : Lambda -> Lambda -> Lambda.
+Module Lambda.
 
-Section LambdaParsing.
+  (* Lambda Calculus with 0-indexed De Bruijn indices *)
+  Inductive Lambda : Set :=
+  | var : nat -> Lambda
+  | out : Lambda -> Lambda
+  | lam : Lambda -> Lambda
+  | app : Lambda -> Lambda -> Lambda.
 
-  Local Inductive LambdaTree : Set :=
-  | lam_end
-  | lam_lam (t: LambdaTree)
-  | lam_dot (t: LambdaTree)
-  | lam_out (t: LambdaTree)
-  | lam_wsp (t: LambdaTree)
-  | lam_id (str: string) (t: LambdaTree)
-  | lam_paren (inner: LambdaTree) (t: LambdaTree).
+  Section LambdaParsing.
 
-  Local Definition ParseState := @Parse.ParseState LambdaTree.
+    Local Inductive LambdaTree : Set :=
+    | lam_end
+    | lam_lam (t: LambdaTree)
+    | lam_dot (t: LambdaTree)
+    | lam_out (t: LambdaTree)
+    | lam_wsp (t: LambdaTree)
+    | lam_id (str: string) (t: LambdaTree)
+    | lam_paren (inner: LambdaTree) (t: LambdaTree).
 
-  Function parse_lambdatree_state (l: list ascii): ParseState :=
-    match l with
-    | [] => Parse.ok lam_end []
-    | hd :: tl =>
-      match parse_lambdatree_state tl with
-      | Parse.error => Parse.error
+    Local Definition ParseState := @Parse.ParseState LambdaTree.
+
+    Function parse_lambdatree_state (l: list ascii): ParseState :=
+      match l with
+      | [] => Parse.ok lam_end []
+      | hd :: tl =>
+        match parse_lambdatree_state tl with
+        | Parse.error => Parse.error
+        | Parse.ok cur stack =>
+          match hd with
+          | "032"%char
+          | "009"%char
+          | "010"%char
+          | "013"%char =>
+            match cur with
+            | lam_wsp _ => Parse.ok cur stack
+            | _ => Parse.ok (lam_wsp cur) stack
+            end
+          | "\"%char => Parse.ok (lam_lam cur) stack
+          | "."%char => Parse.ok (lam_dot cur) stack
+          | "^"%char => Parse.ok (lam_out cur) stack
+          | ")"%char => Parse.ok (lam_end) (cur :: stack)
+          | "("%char =>
+            match stack with
+            | [] => Parse.error
+            | next :: stack' => Parse.ok (lam_paren cur next) stack'
+            end
+          | _ =>
+            match cur with
+            | lam_id str next => Parse.ok (lam_id (String hd str) next) stack
+            | _ => Parse.ok (lam_id (String hd EmptyString) cur) stack
+            end
+          end
+        end
+      end.
+
+    Function lambda_strip_wsp (t: LambdaTree): LambdaTree :=
+      match t with
+      | lam_end => lam_end
+      | lam_wsp t' => lambda_strip_wsp t'
+      | lam_lam t' => lam_lam (lambda_strip_wsp t')
+      | lam_dot t' => lam_dot (lambda_strip_wsp t')
+      | lam_out t' => lam_out (lambda_strip_wsp t')
+      | lam_id s t' => lam_id s (lambda_strip_wsp t')
+      | lam_paren inner t' =>
+        lam_paren (lambda_strip_wsp inner) (lambda_strip_wsp t')
+      end.
+
+    Local Inductive NamedLambda : Set :=
+    | nl_var (s: string)
+    | nl_lam (s: string) (e: NamedLambda)
+    | nl_out (e: NamedLambda)
+    | nl_app (e1: NamedLambda) (e2: NamedLambda).
+
+    Function app_of_lambda_list (ls: list NamedLambda)
+             {measure List.length ls}: option NamedLambda :=
+      match ls with
+      | [] => None
+      | e :: [] => Some e
+      | e1 :: e2 :: tl => app_of_lambda_list ((nl_app e1 e2) :: tl)
+      end.
+    intuition.
+    Defined.
+
+    Function named_lambda_of_tree (acc: list NamedLambda) (t: LambdaTree):
+      option NamedLambda :=
+      match t with
+      | lam_end => app_of_lambda_list (rev acc)
+      | lam_wsp _ => None
+      | lam_lam (lam_id s (lam_dot t')) =>
+        match named_lambda_of_tree [] t' with
+        | None => None
+        | Some e => Some (nl_lam s e)
+        end
+      | lam_lam _ | lam_dot _ => None
+      | lam_out t' =>
+        match named_lambda_of_tree [] t' with
+        | None => None
+        | Some e => Some (nl_out e)
+        end
+      | lam_id s t' => named_lambda_of_tree (nl_var s :: acc) t'
+      | lam_paren inner t' =>
+        match named_lambda_of_tree [] inner with
+        | None => None
+        | Some e => named_lambda_of_tree (e :: acc) t'
+        end
+      end.
+
+    Function parse_named_lambda (s: string): option NamedLambda :=
+      match parse_lambdatree_state (Parse.chars_of_string s) with
+      | Parse.error => None
       | Parse.ok cur stack =>
-        match hd with
-        | "032"%char
-        | "009"%char
-        | "010"%char
-        | "013"%char =>
-          match cur with
-          | lam_wsp _ => Parse.ok cur stack
-          | _ => Parse.ok (lam_wsp cur) stack
-          end
-        | "\"%char => Parse.ok (lam_lam cur) stack
-        | "."%char => Parse.ok (lam_dot cur) stack
-        | "^"%char => Parse.ok (lam_out cur) stack
-        | ")"%char => Parse.ok (lam_end) (cur :: stack)
-        | "("%char =>
-          match stack with
-          | [] => Parse.error
-          | next :: stack' => Parse.ok (lam_paren cur next) stack'
-          end
-        | _ =>
-          match cur with
-          | lam_id str next => Parse.ok (lam_id (String hd str) next) stack
-          | _ => Parse.ok (lam_id (String hd EmptyString) cur) stack
+        match stack with
+        | _ :: _ => None
+        | [] => named_lambda_of_tree [] (lambda_strip_wsp cur)
+        end
+      end.
+
+    Example named_id:
+      parse_named_lambda "\x.x" = Some (nl_lam "x" (nl_var "x")).
+    auto. Qed.
+
+    Example named_true:
+      parse_named_lambda "\x.\y.x" =
+      Some (nl_lam "x" (nl_lam "y" (nl_var "x"))).
+    auto. Qed.
+
+    Example named_false:
+      parse_named_lambda " \ x . \ y  .  (y  ) " =
+      Some (nl_lam "x" (nl_lam "y" (nl_var "y"))).
+    auto. Qed.
+
+    Example named_out:
+      parse_named_lambda "\x.^x" = Some (nl_lam "x" (nl_out (nl_var "x"))).
+    auto. Qed.
+
+    Example named_Y:
+      parse_named_lambda "\f.(\x.f (x x)) (\x.f (x x))" =
+      let fn_app := nl_app (nl_var "f") (nl_app (nl_var "x") (nl_var "x")) in
+      Some (nl_lam "f" (nl_app (nl_lam "x" fn_app) (nl_lam "x" fn_app))).
+    auto. Qed.
+
+    Example named_parens:
+      parse_named_lambda "(((\x.(((x))))))" = Some (nl_lam "x" (nl_var "x")).
+    auto. Qed.
+
+    Example named_apps:
+      parse_named_lambda "x y z w" =
+      Some (nl_app (
+                nl_app (
+                    nl_app (nl_var "x") (nl_var "y")
+                  ) (nl_var "z")
+              ) (nl_var "w")).
+    auto. Qed.
+
+    Example named_bad_lambdas: parse_named_lambda "\\x.x" = None.
+    auto. Qed.
+
+    Example named_bad_dots: parse_named_lambda "\x..x" = None.
+    auto. Qed.
+
+    Example named_bad_parens: parse_named_lambda "\x.((x)" = None.
+    auto. Qed.
+
+    Example named_bad_parens2: parse_named_lambda "\x.x ()" = None.
+    auto. Qed.
+
+    Function index_of (x: string) (l: list string): option nat :=
+      match l with
+      | [] => None
+      | hd :: tl =>
+        if string_dec hd x then Some 0
+        else match index_of x tl with
+             | Some i => Some (S i)
+             | None => None
+             end
+      end.
+
+    Function lambda_strip_names (l: NamedLambda) (xs: list string):
+      option Lambda :=
+      match l with
+      | nl_var x =>
+        match index_of x xs with
+        | Some n => Some (var n)
+        | None => None
+        end
+      | nl_lam x e =>
+        match lambda_strip_names e (x :: xs) with
+        | Some e' => Some (lam e')
+        | None => None
+        end
+      | nl_out e =>
+        match lambda_strip_names e xs with
+        | Some e' => Some (out e')
+        | None => None
+        end
+      | nl_app e1 e2 =>
+        match (lambda_strip_names e1 xs, lambda_strip_names e2 xs) with
+        | (Some e1', Some e2') => Some (app e1' e2')
+        | _ => None
+        end
+      end.
+
+    Function parse_lambda (s: string): option Lambda :=
+      match parse_named_lambda s with
+      | None => None
+      | Some nl => lambda_strip_names nl []
+      end.
+
+    Example lambda_id: parse_lambda "\x.x" = Some (lam (var 0)).
+    auto. Qed.
+
+    Example lambda_true:
+      parse_lambda "\x.\y.x" = Some (lam (lam (var 1))).
+    auto. Qed.
+
+    Example lambda_false:
+      parse_lambda " \ x . \ y  .  (y  ) " =  Some (lam (lam (var 0))).
+    auto. Qed.
+
+    Example lambda_out:
+      parse_lambda "\x.^x" = Some (lam (out (var 0))).
+    auto. Qed.
+
+    Example lambda_Y:
+      parse_lambda "\f.(\x.f (x x)) (\x.f (x x))" =
+      let fn_app := app (var 1) (app (var 0) (var 0)) in
+      Some (lam (app (lam fn_app) (lam fn_app))).
+    auto. Qed.
+
+    Example lambda_parens:
+      parse_lambda "(((\x.(((x))))))" = Some (lam (var 0)).
+    auto. Qed.
+
+    Example lambda_apps:
+      parse_lambda "x y z w" = None.
+    auto. Qed.
+
+  End LambdaParsing.
+
+  Function lambda_replace (e: Lambda) (x: Lambda) (n: nat): Lambda :=
+    match e with
+    | var m => if m =? n then x else e
+    | lam e' => lam (lambda_replace e' x (S n))
+    | out e' => out (lambda_replace e' x n)
+    | app e1 e2 => app (lambda_replace e1 x n) (lambda_replace e2 x n)
+    end.
+
+  Function count_apps (e: Lambda): option nat :=
+    match e with
+    | var 0 => Some 0
+    | app (var 1) e' =>
+      match count_apps e' with
+      | Some n => Some (S n)
+      | None => None
+      end
+    | _ => None
+    end.
+
+  Function nat_of_lambda (e: Lambda): option nat :=
+    match e with
+    | lam (lam e') => count_apps e'
+    | _ => None
+    end.
+
+  (* Call by value semantics *)
+  Function lambda_step (e: Lambda): option (Lambda * option nat) :=
+    match e with
+    | var _ => None
+    | lam e' => None
+    | out e' =>
+      match lambda_step e' with
+      | Some (e'', n) => Some (out e'', n)
+      | None => Some (e', nat_of_lambda e')
+      end
+    | app e1 e2 =>
+      match lambda_step e1 with
+      | Some (e1', n) => Some (app e1' e2, n)
+      | None =>
+        match lambda_step e2 with
+        | Some (e2', n) => Some (app e1 e2', n)
+        | None =>
+          match e1 with
+          | lam e1' => Some (lambda_replace e1' e2 0, None)
+          | _ => None
           end
         end
       end
     end.
 
-  Function lambda_strip_wsp (t: LambdaTree): LambdaTree :=
-    match t with
-    | lam_end => lam_end
-    | lam_wsp t' => lambda_strip_wsp t'
-    | lam_lam t' => lam_lam (lambda_strip_wsp t')
-    | lam_dot t' => lam_dot (lambda_strip_wsp t')
-    | lam_out t' => lam_out (lambda_strip_wsp t')
-    | lam_id s t' => lam_id s (lambda_strip_wsp t')
-    | lam_paren inner t' =>
-      lam_paren (lambda_strip_wsp inner) (lambda_strip_wsp t')
+  Inductive LambdaState :=
+  | l_state (output: list nat) (l: Lambda).
+
+  Function lambda_steps (state: LambdaState) (fuel: nat):
+    (LambdaState * nat) :=
+    match fuel with
+    | 0 => (state, fuel)
+    | S f =>
+      match state with
+      | l_state output e =>
+        match lambda_step e with
+        | Some (e', None) => lambda_steps (l_state output e') f
+        | Some (e', Some n) => lambda_steps (l_state (output ++ [n]) e') f
+        | None => (state, fuel)
+        end
+      end
     end.
 
-  Local Inductive NamedLambda : Set :=
-  | nl_var (s: string)
-  | nl_lam (s: string) (e: NamedLambda)
-  | nl_out (e: NamedLambda)
-  | nl_app (e1: NamedLambda) (e2: NamedLambda).
-
-  Function app_of_lambda_list (ls: list NamedLambda) {measure List.length ls}:
-    option NamedLambda :=
-    match ls with
-    | [] => None
-    | e :: [] => Some e
-    | e1 :: e2 :: tl => app_of_lambda_list ((nl_app e1 e2) :: tl)
+  Function lambda_run (state: LambdaState) (fuel: nat): option LambdaState :=
+    match lambda_steps state fuel with
+    | (_, 0) => None
+    | (state' , _) => Some state'
     end.
-  intuition.
+
+  Inductive LambdaNorm :=
+  | norm (l: Lambda) (term: lambda_step l = None)
+         (no_free: forall l' n, lambda_replace l l' n = l).
+
+  Function get_lam (ln: LambdaNorm): Lambda :=
+    match ln with norm l _ _ => l end.
+
+  Definition l_id: LambdaNorm.
+    refine (norm (lam (var 0)) _ _); auto.
   Defined.
 
-  Function named_lambda_of_tree (acc: list NamedLambda) (t: LambdaTree):
-    option NamedLambda :=
-    match t with
-    | lam_end => app_of_lambda_list (rev acc)
-    | lam_wsp _ => None
-    | lam_lam (lam_id s (lam_dot t')) =>
-      match named_lambda_of_tree [] t' with
-      | None => None
-      | Some e => Some (nl_lam s e)
-      end
-    | lam_lam _ | lam_dot _ => None
-    | lam_out t' =>
-      match named_lambda_of_tree [] t' with
-      | None => None
-      | Some e => Some (nl_out e)
-      end
-    | lam_id s t' => named_lambda_of_tree (nl_var s :: acc) t'
-    | lam_paren inner t' =>
-      match named_lambda_of_tree [] inner with
-      | None => None
-      | Some e => named_lambda_of_tree (e :: acc) t'
-      end
+  Function parse_def (s: string): Lambda :=
+    match parse_lambda s with
+    | Some l => l
+    | None => get_lam l_id
     end.
 
-  Function parse_named_lambda (s: string): option NamedLambda :=
-    match parse_lambdatree_state (Parse.chars_of_string s) with
-    | Parse.error => None
-    | Parse.ok cur stack =>
-      match stack with
-      | _ :: _ => None
-      | [] => named_lambda_of_tree [] (lambda_strip_wsp cur)
-      end
+  Definition ZERO := "(\f.\x.x)"%string.
+  Definition SUCC := "(\n.\f.\x.f (n f x))"%string.
+  Definition TRUE := "(\x.\y.x)"%string.
+  Definition FALSE := "(\x.\y.y)"%string.
+  Definition EMPTY := "(\f.f (\x.\y.x) (\x.x))"%string.
+  Definition CONS := "(\a.\l.\f.f (\x.\y.y) (\f.f a l))"%string.
+  Definition ISEMPTY := "(\l.l (\x.\y.x))"%string.
+  Definition HEAD := "(\l.l (\x.\y.y) (\x.\y.x))"%string.
+  Definition TAIL := "(\l.l (\x.\y.y) (\x.\y.y))"%string.
+  Definition THETA :=
+    "((\x.\y.(y (\z.x x y z))) (\x.\y.(y (\z.x x y z))))"%string.
+
+  Definition l_zero: LambdaNorm.
+    refine (norm (parse_def ZERO) _ _); auto.
+  Defined.
+
+  Definition l_succ: LambdaNorm.
+    refine (norm (parse_def SUCC) _ _); auto.
+  Defined.
+
+  Definition l_true: LambdaNorm.
+    refine (norm (parse_def TRUE) _ _); auto.
+  Defined.
+
+  Definition l_false: LambdaNorm.
+    refine (norm (parse_def FALSE) _ _); auto.
+  Defined.
+
+  Definition l_empty: LambdaNorm.
+    refine (norm (parse_def EMPTY) _ _); auto.
+  Defined.
+
+  Definition l_cons: LambdaNorm.
+    refine (norm (parse_def CONS) _ _); auto.
+  Defined.
+
+  Definition l_isempty: LambdaNorm.
+    refine (norm (parse_def ISEMPTY) _ _); auto.
+  Defined.
+
+  Definition l_head: LambdaNorm.
+    refine (norm (parse_def HEAD) _ _); auto.
+  Defined.
+
+  Definition l_tail: LambdaNorm.
+    refine (norm (parse_def TAIL) _ _); auto.
+  Defined.
+
+  Definition l_theta := parse_def THETA.
+
+  Lemma isempty_correct_emp:
+    exists f,
+      lambda_run (l_state [] (app (get_lam l_isempty) (get_lam l_empty))) f =
+      Some (l_state [] (get_lam l_true)).
+  Proof.
+    exists 10.
+    auto.
+  Qed.
+
+  Lemma isempty_correct_cons (hd tl: LambdaNorm):
+    exists f,
+      lambda_run
+        (l_state [] (app (get_lam l_isempty)
+                         (app (app (get_lam l_cons) (get_lam hd))
+                              (get_lam tl)))) f =
+      Some (l_state [] (get_lam l_false)).
+  Proof.
+    exists 7.
+    destruct hd, tl.
+    unfold lambda_run.
+    simpl.
+    unfold ISEMPTY; simpl.
+    rewrite term.
+    simpl.
+    now rewrite term0.
+  Qed.
+
+  Eval compute in lambda_steps
+        (l_state [] (app (get_lam l_head)
+                         (app (app (get_lam l_cons) (get_lam l_zero))
+                              (get_lam l_empty)))) 9.
+
+  Lemma head_correct (hd tl: LambdaNorm):
+    exists f,
+      lambda_run
+        (l_state [] (app (get_lam l_head)
+                         (app (app (get_lam l_cons) (get_lam hd))
+                              (get_lam tl)))) f =
+      Some (l_state [] (get_lam hd)).
+  Proof.
+    exists 10.
+    destruct hd, tl.
+    unfold lambda_run.
+    simpl.
+    rewrite term.
+    unfold HEAD, CONS; simpl.
+    rewrite term0; simpl.
+    repeat rewrite no_free.
+    repeat rewrite no_free0.
+    rewrite term.
+    simpl.
+    rewrite term0.
+    rewrite no_free.
+    now rewrite term.
+  Qed.
+
+  Lemma tail_correct (hd tl: LambdaNorm):
+    exists f,
+      lambda_run
+        (l_state [] (app (get_lam l_tail)
+                         (app (app (get_lam l_cons) (get_lam hd))
+                              (get_lam tl)))) f =
+      Some (l_state [] (get_lam tl)).
+  Proof.
+    exists 10.
+    destruct hd, tl.
+    unfold lambda_run.
+    simpl.
+    rewrite term.
+    unfold HEAD, CONS; simpl.
+    rewrite term0; simpl.
+    repeat rewrite no_free.
+    repeat rewrite no_free0.
+    rewrite term.
+    simpl.
+    now repeat rewrite term0.
+  Qed.
+
+  Eval compute in lambda_steps (l_state [] (app l_theta (get_lam l_id))) 50.
+  Eval compute in lambda_steps (l_state [] (app l_theta (get_lam l_id))) 0.
+  Eval compute in lambda_steps (l_state [] (app l_theta (get_lam l_id))) 1.
+  Eval compute in lambda_steps (l_state [] (app l_theta (get_lam l_id))) 2.
+  Eval compute in lambda_steps (l_state [] (app l_theta (get_lam l_id))) 3.
+
+
+
+  Lemma theta_correct (g: LambdaNorm):
+    exists f,
+      lambda_steps (l_state [] (app l_theta (get_lam l_id))) f =
+      (l_state [] (app (app (get_lam l_id) l_theta) (get_lam l_id)), 0).
+  Proof.
+    exists 10.
+    simpl.
+
+
+  Function lambda_unfold_nat (n: nat): Lambda :=
+    match n with
+    | 0 => var 0
+    | S n' => app (var 1) (lambda_unfold_nat n')
     end.
 
-  Example named_id: parse_named_lambda "\x.x" = Some (nl_lam "x" (nl_var "x")).
-  auto. Qed.
+  Definition lambda_of_nat (n: nat): Lambda :=
+    lam (lam (lambda_unfold_nat n)).
 
-  Example named_true:
-    parse_named_lambda "\x.\y.x" = Some (nl_lam "x" (nl_lam "y" (nl_var "x"))).
-  auto. Qed.
-
-  Example named_false:
-    parse_named_lambda " \ x . \ y  .  (y  ) " =
-    Some (nl_lam "x" (nl_lam "y" (nl_var "y"))).
-  auto. Qed.
-
-  Example named_out:
-    parse_named_lambda "\x.^x" = Some (nl_lam "x" (nl_out (nl_var "x"))).
-  auto. Qed.
-
-  Example named_Y:
-    parse_named_lambda "\f.(\x.f (x x)) (\x.f (x x))" =
-    let fn_app := nl_app (nl_var "f") (nl_app (nl_var "x") (nl_var "x")) in
-    Some (nl_lam "f" (nl_app (nl_lam "x" fn_app) (nl_lam "x" fn_app))).
-  auto. Qed.
-
-  Example named_parens:
-    parse_named_lambda "(((\x.(((x))))))" = Some (nl_lam "x" (nl_var "x")).
-  auto. Qed.
-
-  Example named_apps:
-    parse_named_lambda "x y z w" =
-    Some (nl_app (
-              nl_app (
-                  nl_app (nl_var "x") (nl_var "y")
-                ) (nl_var "z")
-            ) (nl_var "w")).
-  auto. Qed.
-
-  Example named_bad_lambdas: parse_named_lambda "\\x.x" = None.
-  auto. Qed.
-
-  Example named_bad_dots: parse_named_lambda "\x..x" = None.
-  auto. Qed.
-
-  Example named_bad_parens: parse_named_lambda "\x.((x)" = None.
-  auto. Qed.
-
-  Example named_bad_parens2: parse_named_lambda "\x.x ()" = None.
-  auto. Qed.
-
-  Function index_of (x: string) (l: list string): option nat :=
-    match l with
-    | [] => None
-    | hd :: tl =>
-      if string_dec hd x then Some 0
-      else match index_of x tl with
-           | Some i => Some (S i)
-           | None => None
-           end
+  (* TODO: Reduce before returning *)
+  Function lambda_of_nats (ns: list nat): Lambda :=
+    match ns with
+    | [] => get_lam l_empty
+    | hd :: tl => lam (app (app (var 0) (lam (lam (var 0))))
+                           (lam (app (app (var 0) (lambda_of_nat hd))
+                                     (lambda_of_nats tl))))
     end.
 
-  Function lambda_strip_names (l: NamedLambda) (xs: list string):
-    option Lambda :=
-    match l with
-    | nl_var x =>
-      match index_of x xs with
-      | Some n => Some (l_var n)
-      | None => None
-      end
-    | nl_lam x e =>
-      match lambda_strip_names e (x :: xs) with
-      | Some e' => Some (l_lam e')
-      | None => None
-      end
-    | nl_out e =>
-      match lambda_strip_names e xs with
-      | Some e' => Some (l_out e')
-      | None => None
-      end
-    | nl_app e1 e2 =>
-      match (lambda_strip_names e1 xs, lambda_strip_names e2 xs) with
-      | (Some e1', Some e2') => Some (l_app e1' e2')
-      | _ => None
-      end
-    end.
-
-  Function parse_lambda (s: string): option Lambda :=
-    match parse_named_lambda s with
+  (* The important interpreter as far as the spec is concerned *)
+  Function interpret_lambda (prog: string) (input: list nat) (f: nat):
+    option (list nat) :=
+    match parse_lambda prog with
     | None => None
-    | Some nl => lambda_strip_names nl []
+    | Some l =>
+      match lambda_run (l_state [] (app l (lambda_of_nats input))) f with
+      | None => None
+      | Some (l_state output _) => Some output
+      end
     end.
 
-  Example lambda_id: parse_lambda "\x.x" = Some (l_lam (l_var 0)).
-  auto. Qed.
-
-  Example lambda_true:
-    parse_lambda "\x.\y.x" = Some (l_lam (l_lam (l_var 1))).
-  auto. Qed.
-
-  Example lambda_false:
-    parse_lambda " \ x . \ y  .  (y  ) " =  Some (l_lam (l_lam (l_var 0))).
-  auto. Qed.
-
-  Example lambda_out:
-    parse_lambda "\x.^x" = Some (l_lam (l_out (l_var 0))).
-  auto. Qed.
-
-  Example lambda_Y:
-    parse_lambda "\f.(\x.f (x x)) (\x.f (x x))" =
-    let fn_app := l_app (l_var 1) (l_app (l_var 0) (l_var 0)) in
-    Some (l_lam (l_app (l_lam fn_app) (l_lam fn_app))).
-  auto. Qed.
-
-  Example lambda_parens:
-    parse_lambda "(((\x.(((x))))))" = Some (l_lam (l_var 0)).
-  auto. Qed.
-
-  Example lambda_apps:
-    parse_lambda "x y z w" = None.
-  auto. Qed.
-
-End LambdaParsing.
-
-Function lambda_replace (e: Lambda) (x: Lambda) (n: nat): Lambda :=
-  match e with
-  | l_var m => if m =? n then x else e
-  | l_lam e' => l_lam (lambda_replace e' x (S n))
-  | l_out e' => l_out (lambda_replace e' x n)
-  | l_app e1 e2 => l_app (lambda_replace e1 x n) (lambda_replace e2 x n)
-  end.
-
-Function count_apps (e: Lambda): option nat :=
-  match e with
-  | l_var 0 => Some 0
-  | l_app (l_var 1) e' =>
-    match count_apps e' with
-    | Some n => Some (S n)
-    | None => None
-    end
-  | _ => None
-  end.
-
-Function nat_of_lambda (e: Lambda): option nat :=
-  match e with
-  | l_lam (l_lam e') => count_apps e'
-  | _ => None
-  end.
-
-(* Call by value semantics *)
-Function lambda_step (e: Lambda): (option Lambda * option nat) :=
-  match e with
-  | l_var _ => (None, None)
-  | l_lam e' => (None, None)
-  | l_out e' =>
-    match lambda_step e' with
-    | (Some e'', n) => (Some (l_out e''), n)
-    | (None, None) => (Some e', nat_of_lambda e')
-    | (None, _) => (None, None)
-    end
-  | l_app e1 e2 =>
-    match lambda_step e1 with
-    | (Some e1', n) => (Some (l_app e1' e2), n)
-    | (None, _) =>
-      match lambda_step e2 with
-      | (Some e2', n) => (Some (l_app e1 e2'), n)
-      | (None, _) =>
-        match e1 with
-        | l_lam e1' => (Some (lambda_replace e1' e2 0), None)
-        | _ => (None, None)
-        end
-      end
-    end
-  end.
-
-(* (* non-CBV semantics *) *)
-(* Function lambda_step (e: Lambda): (option Lambda * option nat) := *)
-(*   match e with *)
-(*   | l_var _ => (None, None) *)
-(*   | l_lam e' => *)
-(*     match lambda_step e' with *)
-(*     | (Some e'', n) => (Some (l_lam e''), n) *)
-(*     | (None, _) => (None, None) *)
-(*     end *)
-(*   | l_out e' => *)
-(*     match lambda_step e' with *)
-(*     | (Some e'', n) => (Some (l_out e''), n) *)
-(*     | (None, None) => (Some e', nat_of_lambda e') *)
-(*     | (None, _) => (None, None) *)
-(*     end *)
-(*   | l_app e1 e2 => *)
-(*     match lambda_step e1 with *)
-(*     | (Some e1', n) => (Some (l_app e1' e2), n) *)
-(*     | (None, _) => *)
-(*       match lambda_step e2 with *)
-(*       | (Some e2', n) => (Some (l_app e1 e2'), n) *)
-(*       | (None, _) => *)
-(*         match e1 with *)
-(*         | l_lam e1' => (Some (lambda_replace e1' e2 0), None) *)
-(*         | _ => (None, None) *)
-(*         end *)
-(*       end *)
-(*     end *)
-(*   end. *)
-
-Inductive LambdaState :=
-| lambda_state (output: list nat) (l: Lambda).
-
-(* DEBUGGING! *)
-Function lambda_steps (l: Lambda) (fuel: nat): (Lambda * nat) :=
-  match fuel with
-  | 0 => (l, fuel)
-  | S f =>
-    match lambda_step l with
-    | (Some l', _) => lambda_steps l' f
-    | _ => (l, fuel)
-    end
-  end.
-
-(* TODO: test me *)
-Function lambda_run (state: LambdaState) (fuel: nat): option (list nat) :=
-  match fuel with
-  | 0 => None
-  | S f =>
-    match state with
-    | lambda_state out e =>
-      match lambda_step e with
-      | (Some e', None) => lambda_run (lambda_state out e') f
-      | (Some e', Some n) => lambda_run (lambda_state (out ++ [n]) e') f
-      | (None, _) => Some out
-      end
-    end
-  end.
-
-Definition l_id := l_lam (l_var 0).
-
-Function parse_def (s: string): Lambda :=
-  match parse_lambda s with
-  | Some l => l
-  | None => l_id
-  end.
-
-(* TODO: test/prove these *)
-Definition l_zero := parse_def "\f.\x.x".
-Definition l_succ := parse_def "\n.\f.\x.f (n f x)".
-Definition l_true := parse_def "\x.\y.x".
-Definition l_false := parse_def "\x.\y.y".
-Definition l_empty := parse_def "\f.f (\x.\y.\x) (\x.x)".
-Definition l_cons := parse_def "\a.\l.\f.f (\x.\y.y) (\f.f a l)".
-Definition l_isempty := parse_def "\l.l (\x.\y.x)".
-Definition l_head := parse_def "\l.l (\x.\y.y) (\x.\y.x)".
-Definition l_tail := parse_def "\l.l (\x.\y.y) (\x.\y.y)".
-
-Function lambda_unfold_nat (n: nat): Lambda :=
-  match n with
-  | 0 => l_var 0
-  | S n' => l_app (l_var 1) (lambda_unfold_nat n')
-  end.
-
-Definition lambda_of_nat (n: nat): Lambda :=
-  l_lam (l_lam (lambda_unfold_nat n)).
-
-(* TODO: Reduce before returning *)
-Function lambda_of_nats (ns: list nat): Lambda :=
-  match ns with
-  | [] => l_empty
-  | hd :: tl => l_lam (l_app (l_app (l_var 0) (l_lam (l_lam (l_var 0)))) (l_lam (l_app (l_app (l_var 0) (lambda_of_nat hd)) (lambda_of_nats tl))))
-  end.
-
-(* The important interpreter as far as the spec is concerned *)
-Function interpret_lambda (prog: string) (input: list nat) (f: nat):
-  option (list nat) :=
-  match parse_lambda prog with
-  | None => None
-  | Some l => lambda_run (lambda_state [] (l_app l (lambda_of_nats input))) f
-  end.
+  Eval compute in
+      let prog := parse_def ("\x.(\y.(\x.x)) ^("++HEAD++"("++TAIL++" x))") in
+      lambda_run (l_state [] (app prog (lambda_of_nats [72;60]))) 20.
 
 
-Eval compute in lambda_run (lambda_state [] (l_app (parse_def "\x.^(x (\x.\y.y) (\x.\y.x))") (lambda_of_nats [72]))) 20.
+  Function nats_of_string (str: string): list nat :=
+    match str with
+    | EmptyString => []
+    | String a str' => nat_of_ascii a :: (nats_of_string str')
+    end.
 
+  Function string_of_nats (ns: list nat): string :=
+    match ns with
+    | [] => EmptyString
+    | n :: ns' => String (ascii_of_nat n) (string_of_nats ns')
+    end.
 
-Function nats_of_string (str: string): list nat :=
-  match str with
-  | EmptyString => []
-  | String a str' => nat_of_ascii a :: (nats_of_string str')
-  end.
+  Function interpret_lambda_readable (prog: string) (input: string) (f: nat):
+    string :=
+    match interpret_lambda prog (nats_of_string input) f with
+    | None => EmptyString
+    | Some ns => string_of_nats ns
+    end.
 
-Function string_of_nats (ns: list nat): string :=
-  match ns with
-  | [] => EmptyString
-  | n :: ns' => String (ascii_of_nat n) (string_of_nats ns')
-  end.
+  Eval compute in interpret_lambda "\input.((\head. ^ (head input)) (\l.l (\x.\y.y) (\x.\y.x)))" [72] 100.
 
-Function interpret_lambda_readable (prog: string) (input: string) (f: nat):
-  string :=
-  match interpret_lambda prog (nats_of_string input) f with
-  | None => EmptyString
-  | Some ns => string_of_nats ns
-  end.
+  Eval compute in interpret_lambda_readable "\input.((\head. ^ (head input)) (\l.l (\x.\y.y) (\x.\y.x)))" "!" 100.
 
-Eval compute in parse_named_lambda "\input.((\head. ^ (head input)) \l.(\x.\y.y) (\x.\y.x))".
-
-Eval compute in interpret_lambda "\input.((\head. ^ (head input)) (\l.l (\x.\y.y) (\x.\y.x)))" [72] 100.
-
-Eval compute in interpret_lambda_readable "\input.((\head. ^ (head input)) (\l.l (\x.\y.y) (\x.\y.x)))" "!" 100.
-
-Definition THETA := "((\x.\y.(y (\z.x x y z))) (\x.\y.(y (\z.x x y z))))"%string.
-Definition ISEMPTY := "(\l.l (\x.\y.x))"%string.
-Definition HEAD := "(\l.l (\x.\y.y) (\x.\y.x))"%string.
-Definition TAIL := "(\l.l (\x.\y.y) (\x.\y.y))"%string.
-
-Eval compute in lambda_steps
-                  (l_app (parse_def ("\input." ++
-                                        THETA ++
-                                        "(\f.\l.("++ISEMPTY++" l)" ++
-                                        "(\x.x)" ++
-                                        "((\_.f ("++TAIL++"l)) ^("++HEAD++ "l)))" ++
-                                        "input"))
-                         (lambda_of_nats [0;1]))
-                  0.
-Eval compute in lambda_steps
-                  (l_app (parse_def ("\input." ++
-                                        THETA ++
-                                        "(\f.\l.("++ISEMPTY++" l)" ++
-                                        "(\x.x)" ++
-                                        "((\_.f ("++TAIL++"l)) ^("++HEAD++ "l)))" ++
-                                        "input"))
-                         (lambda_of_nats [0;1]))
-                  1.
-Eval compute in lambda_steps
-                  (l_app (parse_def ("\input." ++
-                                        THETA ++
-                                        "(\f.\l.("++ISEMPTY++" l)" ++
-                                        "(\x.x)" ++
-                                        "((\_.f ("++TAIL++"l)) ^("++HEAD++ "l)))" ++
-                                        "input"))
-                         (lambda_of_nats [0;1]))
-                  2.
-Eval compute in lambda_steps
-                  (l_app (parse_def ("\input." ++
-                                        THETA ++
-                                        "(\f.\l.("++ISEMPTY++" l)" ++
-                                        "(\x.x)" ++
-                                        "((\_.f ("++TAIL++"l)) ^("++HEAD++ "l)))" ++
-                                        "input"))
-                         (lambda_of_nats [0;1]))
-                  3.
-Eval compute in lambda_steps
-                  (l_app (parse_def ("\input." ++
-                                        THETA ++
-                                        "(\f.\l.("++ISEMPTY++" l)" ++
-                                        "(\x.x)" ++
-                                        "((\_.f ("++TAIL++"l)) ^("++HEAD++ "l)))" ++
-                                        "input"))
-                         (lambda_of_nats [0;1]))
-                  4.
-Eval compute in lambda_steps
-                  (l_app (parse_def ("\input." ++
-                                        THETA ++
-                                        "(\f.\l.("++ISEMPTY++" l)" ++
-                                        "(\x.x)" ++
-                                        "((\_.f ("++TAIL++"l)) ^("++HEAD++ "l)))" ++
-                                        "input"))
-                         (lambda_of_nats [0;1]))
-                  5.
-Eval compute in lambda_steps
-                  (l_app (parse_def ("\input." ++
-                                        THETA ++
-                                        "(\f.\l.("++ISEMPTY++" l)" ++
-                                        "(\x.x)" ++
-                                        "((\_.f ("++TAIL++"l)) ^("++HEAD++ "l)))" ++
-                                        "input"))
-                         (lambda_of_nats [0;1]))
-                  6.
-Eval compute in lambda_steps
-                  (l_app (parse_def ("\input." ++
-                                        THETA ++
-                                        "(\f.\l.("++ISEMPTY++" l)" ++
-                                        "(\x.x)" ++
-                                        "((\_.f ("++TAIL++"l)) ^("++HEAD++ "l)))" ++
-                                        "input"))
-                         (lambda_of_nats [0;1]))
-                  7.
-Eval compute in lambda_steps
-                  (l_app (parse_def ("\input." ++
-                                        THETA ++
-                                        "(\f.\l.("++ISEMPTY++" l)" ++
-                                        "(\x.x)" ++
-                                        "((\_.f ("++TAIL++"l)) ^("++HEAD++ "l)))" ++
-                                        "input"))
-                         (lambda_of_nats [0;1]))
-                  8.
-Eval compute in lambda_steps
-                  (l_app (parse_def ("\input." ++
-                                        THETA ++
-                                        "(\f.\l.("++ISEMPTY++" l)" ++
-                                        "(\x.x)" ++
-                                        "((\_.f ("++TAIL++"l)) ^("++HEAD++ "l)))" ++
-                                        "input"))
-                         (lambda_of_nats [0;1]))
-                  9.
-Eval compute in lambda_steps
-                  (l_app (parse_def ("\input." ++
-                                        THETA ++
-                                        "(\f.\l.("++ISEMPTY++" l)" ++
-                                        "(\x.x)" ++
-                                        "((\_.f ("++TAIL++"l)) ^("++HEAD++ "l)))" ++
-                                        "input"))
-                         (lambda_of_nats [0;1]))
-                  10.
-
-
-Eval compute in
-    interpret_lambda_readable
-      ("\input." ++
-         THETA ++
-         "(\f.\l.("++ISEMPTY++" l)" ++
-                "(\x.x)" ++
-                "((\_.f ("++TAIL++"l)) ^("++HEAD++ "l)))" ++
-         "input")
-      "Hello, world!" 20000.
+  Eval compute in
+      lambda_steps
+        (l_state [] (app (parse_def ("\input." ++
+                                     THETA ++
+                                     "(\f.\l.("++ISEMPTY++" l)" ++
+                                     "(\x.x)" ++
+                                     "((\_.f ("++TAIL++"l)) ^("++HEAD++ "l)))" ++
+                                     "input"))
+                         (lambda_of_nats [1;2;3]))) 16.
 
 
 
-Eval compute in interpret_lambda_readable "\input.(\f.\g.(g (\h. f f g h))) (\f.\g.(g (\h. f f g h))) (\f.\l.(l (\x.\y.x)) (\x.x) ((\_.f (l \x.\y.y) (\x.\y.y)) ^ (l (\x.\y.y) (\x.\y.x)))) input" "He" 30000.
 
-(* TODO: Hello world *)
+  Eval compute in interpret_lambda_readable "\input.(\f.\g.(g (\h. f f g h))) (\f.\g.(g (\h. f f g h))) (\f.\l.(l (\x.\y.x)) (\x.x) ((\_.f (l \x.\y.y) (\x.\y.y)) ^ (l (\x.\y.y) (\x.\y.x)))) input" "He" 30000.
+
+  (* TODO: Hello world *)
+
+End Lambda.
